closed SR

process/sessions.v
@@ -31,7 +31,14 @@ Fixpoint flattenT (M : session) : (list part) :=
 
 Definition InT (pt : part) (M : session) : Prop :=
   In pt (flattenT M).
-  
+
+Inductive unfoldP : relation session := 
+  | pc_sub   : forall p P Q M, substitutionP 0 0 0 (p_rec P) P Q -> unfoldP (p <-- (p_rec P) ||| M) (p <-- Q ||| M)
+  | pc_refl  : forall M, unfoldP M M
+  | pc_trans : forall M M' M'', unfoldP M M' -> unfoldP M' M'' -> unfoldP M M''
+  | pc_par1  : forall M M', unfoldP (M ||| M') (M' ||| M)
+  | pc_par2  : forall M M' M'', unfoldP ((M ||| M') ||| M'') (M ||| (M' ||| M'')).
+
 Inductive typ_sess : session -> gtt -> Prop := 
   | t_sess : forall M G, wfgC G ->
                          (forall pt, isgPartsC pt G -> InT pt M) ->
@@ -39,248 +46,6 @@ Inductive typ_sess : session -> gtt -> Prop :=
                          ForallT (fun u P => exists T, projectionC G u T /\ typ_proc nil nil P T /\ (forall n, exists m, guardP n m P)) M ->
                          typ_sess M G.
 
-
-Inductive stepE : relation expr := 
-  | ec_var   : forall n, stepE (e_var n) (e_var n)
-  | ec_val   : forall v, stepE (e_val v) (e_val v)
-  | ec_succ  : forall n, stepE (e_succ (e_val (vnat n))) (e_val (vnat (n+1)))
-  | ec_neg   : forall n, stepE (e_neg (e_val (vint n))) (e_val (vint (-n)))
-  | ec_t_f   :           stepE (e_not (e_val (vbool true))) (e_val (vbool false))
-  | ec_f_t   :           stepE (e_not (e_val (vbool false))) (e_val (vbool true))
-  | ec_gt_t  : forall m n, Z.lt n m -> stepE (e_gt (e_val (vint m)) (e_val (vint n))) (e_val (vbool true)) 
-  | ec_gt_f  : forall m n, Z.le m n -> stepE (e_gt (e_val (vint m)) (e_val (vint n))) (e_val (vbool false))
-  | ec_plus  : forall m n, stepE (e_plus (e_val (vint n)) (e_val (vint m))) (e_val (vint (n + m)))
-  | ec_detl  : forall m n v, stepE m v -> stepE (e_det m n) v
-  | ec_detr  : forall m n v, stepE n v -> stepE (e_det m n) v.
-
-Inductive multi {X : Type} (R : relation X) : relation X :=
-  | multi_refl : forall (x : X), multi R x x 
-  | multi_step : forall (x y z : X), R x y -> multi R y z -> multi R x z.
-  
-Lemma transitive_multi {X : Type} : forall (R : relation X) (x y z : X), multi R x y -> multi R y z -> multi R x z.
-Proof.
-  intros R x y z H.
-  revert z.
-  induction H; intros. easy.
-  specialize(IHmulti z0 H1).
-  specialize(@multi_step X R); intros.
-  apply H2 with (y := y). easy. easy.
-Qed.
-
-Definition stepE_multi := multi stepE.
-   
-Inductive unfoldP : relation process := 
-  | pc_inact : unfoldP p_inact p_inact
-  | pc_var   : forall n, unfoldP (p_var n) (p_var n)
-  | pc_mu    : forall X Y, unfoldP X Y -> unfoldP (p_rec X) (p_rec Y)
-  | pc_ite   : forall e X X' Y Y', unfoldP X X' -> unfoldP Y Y' -> unfoldP (p_ite e X Y) (p_ite e X' Y')
-  | pc_recv  : forall pt xs ys, Forall2 (fun u v => (u = None /\ v = None) \/ (exists P Q, u = Some P /\ v = Some Q /\ unfoldP P Q)) xs ys -> unfoldP (p_recv pt xs) (p_recv pt ys)
-  | pc_send  : forall pt lb e X X', unfoldP X X' -> unfoldP (p_send pt lb e X) (p_send pt lb e X')
-  | pc_sub   : forall P Q, substitutionP 0 0 0 (p_rec P) P Q -> unfoldP (p_rec P) Q
-  | pc_trans : forall P Q R, unfoldP P Q -> unfoldP Q R -> unfoldP P R.
-
-Section unfoldP_ind_ref.
-  Variable P : process -> process -> Prop.
-  Hypothesis P_inact : P p_inact p_inact.
-  Hypothesis P_var   : forall n, P (p_var n) (p_var n).
-  Hypothesis P_mu    : forall X Y, P X Y -> P (p_rec X) (p_rec Y).
-  Hypothesis P_ite   : forall e X X' Y Y', P X X' -> P Y Y' -> P (p_ite e X Y) (p_ite e X' Y').
-  Hypothesis P_recv  : forall pt xs ys, Forall2 (fun u v => (u = None /\ v = None) \/ (exists X Y, u = Some X /\ v = Some Y /\ P X Y)) xs ys -> P (p_recv pt xs) (p_recv pt ys).
-  Hypothesis P_send  : forall pt lb e X X', P X X' -> P (p_send pt lb e X) (p_send pt lb e X').
-  Hypothesis P_sub   : forall X Y, substitutionP 0 0 0 (p_rec X) X Y -> P (p_rec X) Y.
-  Hypothesis P_trans : forall X Y Z, P X Y -> P Y Z -> P X Z.
-  
-  Fixpoint unfoldP_ind_ref (X Y : process) (a : unfoldP X Y) {struct a} : P X Y.
-  Proof.
-    refine (match a with
-      | pc_inact => P_inact
-      | pc_var n => P_var n 
-      | pc_mu X Y Hp => P_mu X Y (unfoldP_ind_ref X Y Hp)
-      | pc_ite e X X' Y Y' Hx Hy => P_ite e X X' Y Y' (unfoldP_ind_ref X X' Hx) (unfoldP_ind_ref Y Y' Hy)
-      | pc_recv pt xs ys Ha => P_recv pt xs ys _
-      | pc_send pt lb e X X' Hx => P_send pt lb e X X' (unfoldP_ind_ref X X' Hx)
-      | pc_sub X Y Hs => P_sub X Y Hs
-      | pc_trans X Y Z Hxy Hyz => P_trans X Y Z (unfoldP_ind_ref X Y Hxy) (unfoldP_ind_ref Y Z Hyz)
-    end); try easy.
-    revert Ha. apply Forall2_mono. intros.
-    destruct H. left. easy.
-    destruct H. destruct H. destruct H. destruct H0. subst. right.
-    exists x0. exists x1. split; try easy. split; try easy.
-    apply unfoldP_ind_ref; try easy.
-  Qed.
-End unfoldP_ind_ref.
-
-Inductive scong: relation session :=
-  | sc_multi: forall p P Q M, unfoldP P Q -> scong (p <-- P ||| M) (p <-- Q ||| M) 
-  | sc_par1 : forall p M, scong (p <-- p_inact ||| M) M
-  | sc_par2 : forall M M', scong (M ||| M') (M' ||| M)
-  | sc_par3 : forall M M' M'', scong ((M ||| M') ||| M'') (M ||| (M' ||| M'')).
-
-
-
-Lemma expr_typ_step : forall Gs e e' S, typ_expr Gs e S -> stepE e e' -> typ_expr Gs e' S.
-Proof.
-  intros. revert H. revert S. induction H0; intros; try easy.
-  - specialize(inv_expr_succ Gs (e_succ (e_val (vnat n))) S (e_val (vnat n)) H (eq_refl (e_succ (e_val (vnat n))))); intros.
-    destruct H0. destruct H1; subst.
-    apply sc_valn.
-    apply sc_sub with (s := snat). apply sc_valn. apply sni.
-  - specialize(inv_expr_neg Gs (e_neg (e_val (vint n))) S (e_val (vint n)) H (eq_refl (e_neg (e_val (vint n))))); intros.
-    destruct H0. subst. apply sc_vali.
-  - specialize(inv_expr_not Gs (e_not (e_val (vbool true))) S (e_val (vbool true)) H (eq_refl (e_not (e_val (vbool true))))); intros.
-    destruct H0. subst. apply sc_valb.
-    specialize(inv_expr_not Gs (e_not (e_val (vbool false))) S (e_val (vbool false)) H (eq_refl (e_not (e_val (vbool false))))); intros.
-    destruct H0. subst. apply sc_valb.
-  - specialize(inv_expr_gt Gs (e_gt (e_val (vint m)) (e_val (vint n))) S (e_val (vint m)) (e_val (vint n)) H0 (eq_refl (e_gt (e_val (vint m)) (e_val (vint n))))); intros.
-    destruct H1. destruct H2. subst. apply sc_valb.
-  - specialize(inv_expr_gt Gs (e_gt (e_val (vint m)) (e_val (vint n))) S (e_val (vint m)) (e_val (vint n)) H0 (eq_refl (e_gt (e_val (vint m)) (e_val (vint n))))); intros.
-    destruct H1. destruct H2. subst. apply sc_valb.
-  - specialize(inv_expr_plus Gs (e_plus (e_val (vint n)) (e_val (vint m))) S (e_val (vint n)) (e_val (vint m)) H (eq_refl (e_plus (e_val (vint n)) (e_val (vint m))))); intros.
-    destruct H0. destruct H1. subst. apply sc_vali.
-  - specialize(inv_expr_det Gs (e_det m n) S m n H (eq_refl (e_det m n))); intros.
-    destruct H1. destruct H1. destruct H2.
-    apply sc_sub with (s := x); intros; try easy. apply IHstepE; try easy.
-  - specialize(inv_expr_det Gs (e_det m n) S m n H (eq_refl (e_det m n))); intros.
-    destruct H1. destruct H1. destruct H2.
-    apply sc_sub with (s := x); intros; try easy. apply IHstepE; try easy.
-Qed.
-
-
-Lemma expr_typ_multi : forall Gs e e' S, typ_expr Gs e S -> stepE_multi e e' -> typ_expr Gs e' S.
-Proof.
-  intros. revert H. revert S. induction H0; intros; try easy.
-  apply IHmulti.
-  apply expr_typ_step with (e := x); try easy.
-Qed.
-  
-Lemma _a22_2_helperP_1 : forall xs x l' Gs Gt,
-      Forall2
-       (fun u v : option process =>
-        u = None /\ v = None \/
-        (exists X Y : process,
-           u = Some X /\
-           v = Some Y /\
-           (forall (Gs : ctxS) (Gt : ctxT) (T : ltt), typ_proc Gs Gt X T -> typ_proc Gs Gt Y T))) xs l' ->
-      Forall2
-        (fun (u : option process) (v : option (sort * ltt)) =>
-         u = None /\ v = None \/
-         (exists (p : process) (s : sort) (t : ltt),
-            u = Some p /\ v = Some (s, t) /\ typ_proc (Some s :: Gs) Gt p t)) xs x ->
-      Forall2
-      (fun (u : option process) (v : option (sort * ltt)) =>
-       u = None /\ v = None \/
-       (exists (p : process) (s : sort) (t : ltt),
-          u = Some p /\ v = Some (s, t) /\ typ_proc (Some s :: Gs) Gt p t)) l' x.
-Proof.
-  intro xs. induction xs; intros; try easy.
-  inversion H. subst. inversion H0. subst. easy.
-  inversion H. subst. inversion H0. subst. clear H H0.
-  constructor. destruct H3. left. destruct H4; try easy.
-  destruct H. destruct H0. destruct H0. destruct H0. destruct H0. subst. easy.
-  right. destruct H. destruct H. destruct H. destruct H0. subst.
-  exists x0. destruct H4. easy. destruct H. destruct H. destruct H. destruct H. destruct H0. subst.
-  exists x2. exists x3. split; try easy. split; try easy.
-  apply H1. inversion H. subst. easy.
-  apply IHxs; try easy.
-Qed.
-
-Lemma _a22_2_helperP_2 : forall xs l',
-      SList xs ->
-      Forall2
-       (fun u v : option process =>
-        u = None /\ v = None \/
-        (exists X Y : process,
-           u = Some X /\
-           v = Some Y /\
-           (forall (Gs : ctxS) (Gt : ctxT) (T : ltt), typ_proc Gs Gt X T -> typ_proc Gs Gt Y T))) xs l' ->
-      SList l'.
-Proof.
-  intro xs. induction xs; intros; try easy.
-  inversion H0. subst. 
-  specialize(SList_f a xs H); intros. destruct H1.
-  - apply SList_b. apply IHxs; try easy.
-  - destruct H1. destruct H2. subst. inversion H5. subst. destruct H3; try easy.
-    destruct H1. destruct H1. destruct H1. destruct H2. subst. easy.
-Qed.
-  
-Lemma _a22_2_helperP_h : forall Gs Gt pt xs ys T,
-    typ_proc Gs Gt (p_recv pt xs) T ->
-    Forall2
-      (fun u v : option process =>
-       u = None /\ v = None \/
-       (exists X Y : process,
-          u = Some X /\
-          v = Some Y /\
-          (forall (Gs : ctxS) (Gt : ctxT) (T : ltt), typ_proc Gs Gt X T -> typ_proc Gs Gt Y T))) xs ys ->
-    typ_proc Gs Gt (p_recv pt ys) T.
-Proof.
-  intros Gs Gt pt xs. revert Gs Gt pt.
-  induction xs; intros; try easy.
-  - inversion H0. subst. easy.
-  - inversion H0. subst. clear H0.
-    specialize(_a23_a pt (a :: xs) (p_recv pt (a :: xs)) Gs Gt T H (eq_refl (p_recv pt (a :: xs)))); intros.
-    destruct H0. destruct H0. destruct H1. destruct H2.
-    apply tc_sub with (t := ltt_recv pt x); try easy.
-    destruct x; try easy.
-    apply tc_recv; try easy.
-    simpl. apply eq_S.
-    inversion H0.
-    specialize(Forall2_length H5); intros. easy.
-    specialize(SList_f a xs H4); intros. clear H4. destruct H6.
-    - apply SList_b.
-      apply _a22_2_helperP_2 with (xs := xs); try easy.
-    - destruct H4. destruct H6. subst. destruct H3; try easy.
-      destruct H3. destruct H3. destruct H3. destruct H4. inversion H3. subst.
-      inversion H5. subst. easy.
-    - constructor. 
-      destruct H3. left. destruct H3. inversion H2. subst.
-      destruct H10. easy. destruct H3. destruct H3. destruct H3. easy.
-      right.
-      destruct H3. destruct H3. destruct H3. destruct H6. 
-      exists x1.
-      inversion H2; subst. destruct H11; try easy.
-      destruct H3. destruct H3. destruct H3. destruct H3. destruct H6. subst.
-      exists x3. exists x4.
-      split; try easy. split; try easy. 
-      apply H7. inversion H3. subst. easy.
-    - inversion H2. subst. clear H2.
-      apply _a22_2_helperP_1 with (xs := xs); try easy.
-      apply typable_implies_wfC with (P := (p_recv pt (a :: xs))) (Gs := Gs) (Gt := Gt); try easy.
-Qed.
-
-Lemma _a22_1 : forall Gs Gt P Q T, typ_proc Gs Gt P T -> unfoldP P Q -> typ_proc Gs Gt Q T.
-Proof.
-  intros. revert H. revert Gs Gt T.
-  induction H0 using unfoldP_ind_ref; intros; try easy.
-  - specialize(_a23_d (p_rec X) X T Gs Gt H (eq_refl (p_rec X))); intros.
-    destruct H0. destruct H0. 
-    specialize(IHunfoldP Gs (Some x :: Gt) x H0).
-    apply tc_sub with (t := x); try easy.
-    apply tc_mu; try easy.
-    apply typable_implies_wfC with (P := p_rec X) (Gs := Gs) (Gt := Gt); try easy.
-  - specialize(_a23_c (p_ite e X Y) e X Y T Gs Gt H (eq_refl (p_ite e X Y))); intros.
-    destruct H0. destruct H0. destruct H0. destruct H1. destruct H2. destruct H3.
-    apply tc_ite. easy.
-    apply IHunfoldP; try easy. apply tc_sub with (t := x); try easy.
-    apply typable_implies_wfC with (P := p_ite e X Y) (Gs := Gs) (Gt := Gt); try easy.
-    apply IHunfoldP0; try easy. apply tc_sub with (t := x0); try easy.
-    apply typable_implies_wfC with (P := p_ite e X Y) (Gs := Gs) (Gt := Gt); try easy.
-  - apply _a22_2_helperP_h with (xs := xs); try easy.
-  - specialize(_a23_bf pt lb e X (p_send pt lb e X) Gs Gt T H (eq_refl (p_send pt lb e X))); intros.
-    destruct H0. destruct H0. destruct H0. destruct H1.
-    apply tc_sub with (t := (ltt_send pt (extendLis lb (Some (x, x0))))); try easy.
-    apply tc_send; try easy.
-    apply IHunfoldP; try easy.
-    apply typable_implies_wfC with (P := p_send pt lb e X) (Gs := Gs) (Gt := Gt). easy.
-  - specialize(_a23_d (p_rec X) X T Gs Gt H0 (eq_refl (p_rec X))); intros.
-    destruct H1. destruct H1.  
-    specialize(_a21f X (p_rec X)); intros.
-    apply tc_sub with (t := x); intros; try easy.
-    apply H3 with (T := x); try easy.
-    apply tc_mu; intros; try easy.
-    apply typable_implies_wfC with (P := p_rec X) (Gs := Gs) (Gt := Gt); try easy.
-  - apply IHunfoldP0; try easy. apply IHunfoldP; try easy.
-Qed.
 
 Lemma noin_mid {A} : forall (l1 l2 : list A) a a0, ~ In a0 (l1 ++ a :: l2) -> ~ In a0 (l1 ++ l2) /\ a <> a0.
 Proof.
@@ -347,30 +112,28 @@ Proof.
   destruct H0. left. easy. right. apply IHl2; try easy.
 Qed.
 
-Lemma guardP_after_unf : forall P Q,
-    (forall n : fin, exists m : fin, guardP n m P) -> 
-    (unfoldP P Q) -> 
-    (forall n : fin, exists m : fin, guardP n m Q).
-Admitted.
 
-Lemma _a22_2 : forall M M' G, typ_sess M G -> scong M M' -> typ_sess M' G.
+Lemma _a22_2 : forall M M' G, typ_sess M G -> unfoldP M M' -> typ_sess M' G.
 Proof.
   intros. revert H. revert G. induction H0; intros; try easy.
-  - inversion H0. subst.
+  - inversion H0. subst. 
     inversion H4. subst. clear H4. inversion H7. subst. clear H7. 
     apply t_sess; try easy. constructor; try easy. constructor; try easy.
     destruct H5. exists x. split; try easy. destruct H4. split.
-    apply _a22_1 with (P := P); try easy.
-    destruct H5.
-    specialize(guardP_after_unf P Q); intros. apply H7; try easy.
-  - inversion H. subst. inversion H3. subst. clear H3.
-    inversion H6. subst. clear H6. destruct H4. destruct H3.
-    apply t_sess; try easy. destruct H4 as (H4, Ht).
-    specialize(_a23_f p_inact x nil nil H4 (eq_refl p_inact)); intros. subst.
-    unfold InT in *. simpl in *. specialize(H1 pt H6).
-    specialize(pmergeCR G p H0 H3); intros. 
-    destruct H1; try easy. subst. specialize(H5 H6). easy.
-    simpl in H2. inversion H2. subst. easy.
+    destruct H5 as (H5, H6).
+    - specialize(_a23_d (p_rec P) P x nil nil H5 (eq_refl (p_rec P))); intros.
+      destruct H7 as (T,(Ha,Hb)).
+      specialize(_a21f P (p_rec P) T T nil nil Q Ha H); intros.
+      specialize(typable_implies_wfC H5); intros.
+      apply tc_sub with (t := T); try easy.
+      apply H7. apply tc_mu; try easy.
+      destruct H5.
+      intros. specialize(H6 n). destruct H6.
+      inversion H6.
+      - subst. exists 0. constructor.
+      - subst. 
+        specialize(inj_substP H9 H); intros. subst. exists m. easy.
+  - apply IHunfoldP2. apply IHunfoldP1. easy.
   - inversion H. subst. inversion H3. subst. clear H3.
     apply t_sess; try easy.
     - intros. specialize(H1 pt H3).
@@ -393,3 +156,81 @@ Proof.
 
     constructor. easy. constructor; try easy.
 Qed.
+
+
+Inductive stepE : relation expr := 
+  | ec_succ  : forall e n, stepE e (e_val (vnat n)) -> stepE (e_succ e) (e_val (vnat (n+1)))
+  | ec_neg   : forall e n, stepE e (e_val (vint n)) -> stepE (e_neg e) (e_val (vint (-n)))
+  | ec_t_f   : forall e,   stepE e (e_val (vbool true)) -> stepE (e_not e) (e_val (vbool false))
+  | ec_f_t   : forall e,   stepE e (e_val (vbool false)) -> stepE (e_not e) (e_val (vbool true))
+  | ec_gt_t  : forall e e' m n, Z.lt n m -> 
+                           stepE e (e_val (vint m)) -> stepE e' (e_val (vint n)) ->
+                           stepE (e_gt e e') (e_val (vbool true)) 
+  | ec_gt_f  : forall e e' m n, Z.le m n -> 
+                           stepE e (e_val (vint m)) -> stepE e' (e_val (vint n)) ->
+                           stepE (e_gt e e') (e_val (vbool true)) 
+  | ec_plus  : forall e e' m n, stepE e (e_val (vint n)) -> stepE e' (e_val (vint m)) -> 
+                           stepE (e_plus e e') (e_val (vint (n + m)))
+  | ec_detl  : forall m n v, stepE m v -> stepE (e_det m n) v
+  | ec_detr  : forall m n v, stepE n v -> stepE (e_det m n) v
+  | ec_refl  : forall e, stepE e e
+  | ec_trans : forall e e' e'', stepE e e' -> stepE e' e'' -> stepE e e''.
+
+   
+Lemma expr_typ_step : forall Gs e e' S, typ_expr Gs e S -> stepE e e' -> typ_expr Gs e' S.
+Proof.
+  intros. revert H. revert S. induction H0; intros; try easy.
+  - specialize(inv_expr_succ Gs (e_succ e) S e H (eq_refl (e_succ e))); intros.
+    destruct H1. destruct H2; subst.
+    apply sc_valn.
+    apply sc_sub with (s := snat). apply sc_valn. apply sni.
+  - specialize(inv_expr_neg Gs (e_neg e) S e H (eq_refl (e_neg e))); intros.
+    destruct H1. subst. apply sc_vali.
+  - specialize(inv_expr_not Gs (e_not e) S e H (eq_refl (e_not e))); intros.
+    destruct H1. subst. apply sc_valb.
+    specialize(inv_expr_not Gs (e_not e) S e H (eq_refl (e_not e))); intros.
+    destruct H1. subst. apply sc_valb.
+  - specialize(inv_expr_gt Gs (e_gt e e') S e e' H0 (eq_refl (e_gt e e'))); intros.
+    destruct H1. destruct H2. subst. apply sc_valb.
+  - specialize(inv_expr_gt Gs (e_gt e e') S e e' H0 (eq_refl (e_gt e e'))); intros.
+    destruct H1. destruct H2. subst. apply sc_valb.
+  - specialize(inv_expr_plus Gs (e_plus e e') S e e' H (eq_refl (e_plus e e'))); intros.
+    destruct H0. destruct H1. subst. apply sc_vali.
+  - specialize(inv_expr_det Gs (e_det m n) S m n H (eq_refl (e_det m n))); intros.
+    destruct H1. destruct H1. destruct H2.
+    apply sc_sub with (s := x); intros; try easy. apply IHstepE; try easy.
+  - specialize(inv_expr_det Gs (e_det m n) S m n H (eq_refl (e_det m n))); intros.
+    destruct H1. destruct H1. destruct H2.
+    apply sc_sub with (s := x); intros; try easy. apply IHstepE; try easy.
+  - specialize(IHstepE1 S H). specialize(IHstepE2 S). apply IHstepE2; try easy.
+Qed.
+(* 
+Lemma expr_eval_
+
+Lemma expr_eval_b : forall e, typ_expr nil e sbool -> (stepE e (e_val (vbool true)) \/ stepE e (e_val (vbool false))).
+Proof.
+  induction e; intros; try easy.
+  - specialize(inv_expr_var (e_var n) n nil sbool H (eq_refl (e_var n))); intros.
+    destruct H0 as (S',(Ha,Hb)). destruct n; try easy.
+  - specialize(inv_expr_vali nil (e_val v) sbool v H (eq_refl (e_val v))); intros.
+    destruct H0.
+    - destruct H0 as (k,(Ha,Hb)). easy.
+    - destruct H0. destruct H0 as (k,(Ha,Hb)). inversion Ha.
+    - destruct H0 as (k,(Ha,Hb)). subst. destruct k. left. apply ec_refl. right. apply ec_refl. 
+  - specialize(inv_expr_succ nil (e_succ e) sbool e H (eq_refl (e_succ e))); intros.
+    destruct H0 as (H0,H1). destruct H1. easy. easy.
+  - specialize(inv_expr_neg nil (e_neg e) sbool e H (eq_refl (e_neg e))); intros.
+    easy.
+  - specialize(inv_expr_not nil (e_not e) sbool e H (eq_refl (e_not e))); intros.
+    destruct H0.
+    specialize(IHe H1).
+    destruct IHe. right. constructor; try easy.
+    left. constructor; try easy.
+  - specialize(inv_expr_gt nil (e_gt e1 e2) sbool e1 e2 H (eq_refl (e_gt e1 e2))); intros.
+    destruct H0 as (Ha,(Hb,Hc)).
+    
+     apply multi_step with (y := (e_val (vbool false))). constructor. easy.
+Admitted.
+
+
+ *)
