process/subject_reduction.v
@@ -288,13 +288,176 @@ Proof.
     subst. exists x. inversion H4. subst. constructor; try easy.
 Qed. 
 
+Inductive peq_w : process -> process -> Prop := 
+  | peq_var : forall n, peq_w (p_var n) (p_var n)
+  | peq_inact : peq_w p_inact p_inact
+  | peq_send : forall pt lb e e' p1 p2, peq_w p1 p2 -> peq_w (p_send pt lb e p1) (p_send pt lb e' p2)
+  | peq_recv : forall pt xs ys, Forall2 (fun u v => (u = None /\ v = None) \/ (exists p p', u = Some p /\ v = Some p' /\ peq_w p p')) xs ys -> peq_w (p_recv pt xs) (p_recv pt ys)
+  | peq_ite  : forall e1 p1 q1 e2 p2 q2, peq_w p1 p2 -> peq_w q1 q2 -> peq_w (p_ite e1 p1 q1) (p_ite e2 p2 q2)
+  | peq_rec : forall p1 p2, peq_w p1 p2 -> peq_w (p_rec p1) (p_rec p2).
+
+Lemma peq_after_incr : forall g p0 m n k l,
+        peq_w g p0 -> 
+        peq_w (incr_free m n k l g) (incr_free m n k l p0).
+Proof.
+  induction g using process_ind_ref; intros; try easy.
+  - inversion H. subst. constructor.
+  - inversion H. subst. constructor.
+  - inversion H. subst. constructor; try easy. apply IHg; try easy.
+  - inversion H0. subst. constructor; try easy.
+    revert H4 H. clear H0. revert llp m n k l.
+    induction ys; intros; try easy.
+    - destruct llp; try easy.
+    - destruct llp; try easy.
+      inversion H. subst. clear H. inversion H4. subst. clear H4.
+      specialize(IHys llp m n k l H7 H3). constructor; try easy. clear IHys H3 H7.
+      destruct H5.
+      - destruct H. subst. left. easy.
+      - destruct H as (p1,(p2,(Ha,(Hb,Hc)))). subst.
+        right. exists (incr_free m (S n) k l p1). exists (incr_free m (S n) k l p2). split. easy.
+        split. easy.
+        apply H2; try easy.
+  - inversion H. subst. constructor. apply IHg1; try easy. apply IHg2; try easy.
+  - inversion H. subst. constructor. apply IHg; try easy.
+Qed.
+
+Lemma peq_after_subst : forall g1 g Q m n k p0 p1,
+        substitutionP m n k g g1 Q -> 
+        peq_w g p0 -> peq_w g1 p1 ->
+        exists Q' : process, substitutionP m n k p0 p1 Q' /\ peq_w Q Q'.
+Proof.
+  induction g1 using process_ind_ref; intros.
+  - inversion H1. subst.
+    inversion H. subst.
+    - exists (incr_free 0 0 n0 k p0). split. constructor. 
+      apply peq_after_incr; try easy.
+    - subst. exists (p_var 0). split. constructor. easy. constructor.
+    - subst. exists (p_var y). split. constructor; try easy. constructor.
+    - subst. exists (p_var (S y)). split. constructor; try easy. constructor.
+  - inversion H1. subst. 
+    inversion H. subst. exists p_inact. split. constructor. constructor.
+  - inversion H1. subst.
+    inversion H. subst.
+    specialize(IHg1 g Q' m n k p0 p3 H12 H0 H7). destruct IHg1 as (q1,(Ha,Hb)).
+    exists (p_send pt lb e' q1). split. constructor; try easy. constructor; try easy.
+  - inversion H2. subst. inversion H0. subst.
+    clear H2 H0.
+    assert(exists ys3, Forall2 (fun u v => (u = None /\ v = None) \/ (exists p p', u = Some p /\ v = Some p' /\ substitutionP m n (S k) p0 p p')) ys ys3 /\ Forall2 (fun u v => (u = None /\ v = None) \/ (exists p p', u = Some p /\ v = Some p' /\ peq_w p p')) ys0 ys3).
+    {
+      revert H11 H6 H1 H.
+      revert llp g m n k p0 ys0.
+      induction ys; intros.
+      - destruct llp; try easy. destruct ys0; try easy. exists nil. easy.
+      - destruct llp; try easy. destruct ys0; try easy.
+        inversion H11. subst. clear H11. inversion H6. subst. clear H6.
+        inversion H. subst. clear H.
+        specialize(IHys llp g m n k p0 ys0 H7 H9 H1 H6).
+        clear H6 H9 H7.
+        destruct IHys as (ys3,(Ha,Hb)).
+        destruct H4.
+        - destruct H. subst. destruct H5. destruct H. subst.
+          exists (None :: ys3). split. constructor; try easy. left. easy. constructor; try easy. left. easy. 
+          destruct H as (p1,(p2,Hc)). easy.
+        - destruct H as (k1,(l1,(Hc,(Hd,He)))). subst.
+          destruct H5; try easy. destruct H as (p1,(p2,(Hf,(Hg,Hh)))). inversion Hf. subst.
+          specialize(H3 g l1 m n (S k) p0 p2 He H1 Hh).
+          destruct H3 as (q1,(Hg,Hi)).
+          exists (Some q1 :: ys3).
+          - split. constructor; try easy. right. exists p2. exists q1. easy.
+          - constructor; try easy. right. exists l1. exists q1. easy.
+    }
+    destruct H0 as (ys3,(Ha,Hb)). exists (p_recv pt ys3).
+    split. constructor; try easy. constructor; try easy. 
+  - inversion H1. subst. inversion H. subst.
+    specialize(IHg1_1 g Q1 m n k p0 p3 H12 H0 H6). destruct IHg1_1 as (q1,(Ha,Hb)).
+    specialize(IHg1_2 g Q2 m n k p0 q2 H13 H0 H7). destruct IHg1_2 as (q3,(Hc,Hd)).
+    exists (p_ite e2 q1 q3). split. constructor; try easy. constructor; try easy.
+  - inversion H1. subst. inversion H. subst.
+    specialize(IHg1 g Q' (S m) (S n) k p0 p3 H8 H0 H3).
+    destruct IHg1 as (q1,(Ha,Hb)). exists (p_rec q1).
+    split. constructor; try easy.
+    constructor; try easy.
+Qed.
+
+Lemma guardP_peq_w : forall p1 p2, 
+      peq_w p1 p2 -> 
+      (forall n : fin, exists m : fin, guardP n m p1) -> 
+      (forall n : fin, exists m : fin, guardP n m p2).
+Proof.
+  intros.
+  specialize(H0 n). destruct H0 as (m, H0). exists m.
+  revert H0 H. revert p1 p2 m.
+  induction n; intros; try easy.
+  - constructor.
+  - revert IHn H H0. revert n p1 p2.
+    induction m; intros; try easy.
+    inversion H0.
+    - subst. inversion H. subst. constructor.
+    - subst. inversion H. subst. constructor. apply IHn with (p1 := g); try easy.
+    - subst. inversion H. subst.
+      constructor. revert H5 H2 IHn. clear H0 H. revert ys. induction lis; intros; try easy.
+      - destruct ys; try easy.
+      - destruct ys; try easy. inversion H2. subst. clear H2. inversion H5. subst. clear H5.
+        specialize(IHlis ys H7 H3 IHn). constructor; try easy.
+        clear IHlis H3 H7.
+        destruct H4. left. easy.
+        destruct H as (p1,(p2,(Ha,(Hb,Hc)))). subst.
+        destruct H1; try easy. destruct H as (g1,(Hd,He)). inversion Hd. subst.
+        right. exists p2. split. easy. apply IHn with (p1 := g1); try easy.
+    assert(forall (p1 p2 : process),
+      peq_w p1 p2 -> guardP (S n) m p1 -> guardP (S n) m p2).
+    {
+      intros. specialize(IHm n p0 p3). apply IHm; try easy.
+    }
+    inversion H0. subst.
+    - inversion H. constructor.
+    - subst. inversion H. subst. constructor. apply IHn with (p1 := g); try easy.
+    - subst. inversion H. subst. constructor.
+      revert H6 H3. clear H0 H. revert ys.
+      induction lis; intros.
+      - destruct ys; try easy.
+      - destruct ys; try easy. inversion H6. subst. clear H6. inversion H3. subst. clear H3.
+        specialize(IHlis ys H7 H5). constructor; try easy.
+        destruct H4. left. easy.
+        destruct H as (p1,(p2,(Ha,(Hb,Hc)))). subst.
+        destruct H2; try easy. destruct H as (g1,(Hd,He)). inversion Hd. subst.
+        right. exists p2. split. easy.
+        apply IHn with (p1 := g1); try easy.
+    - subst. inversion H. subst.
+      constructor. apply H1 with (p1 := P); try easy. apply H1 with (p1 := Q); try easy.
+    - subst. inversion H. subst.
+      assert(exists Q', substitutionP 0 0 0 (p_rec p0) p0 Q' /\ peq_w Q Q').
+      {
+        apply peq_after_subst with (g1 := g) (g := p_rec g); try easy.
+      }
+      destruct H2 as (Q1,(Ha,Hb)).
+      apply gp_rec with (Q := Q1); try easy.
+      apply H1 with (p1 := Q); try easy.
+Qed.
+
 Lemma guardP_subst_expr : forall y v j k,
     (forall n : fin, exists m : fin, guardP n m y) -> 
     (forall n : fin, exists m : fin, guardP n m (subst_expr_proc y v j k)).
 Proof.
+  intros.
+  apply guardP_peq_w with (p1 := y); try easy.
+  clear H n. revert v j k.
   induction y using process_ind_ref; intros; try easy.
-  - 
-Admitted.
+  - simpl. constructor.
+  - simpl. constructor.
+  - simpl. constructor. apply IHy; try easy.
+  - simpl. constructor.
+    revert H. revert pt v j k. induction llp; intros; try easy.
+    - inversion H. subst. clear H. specialize(IHllp pt v j k H3). constructor; try easy.
+      clear H3 IHllp.
+      destruct a.
+      - right. exists p. exists (subst_expr_proc p v (S j) (S k)). split. easy. split. easy.
+        apply H2; try easy.
+      - left. easy.
+  - simpl. constructor.
+    apply IHy1. apply IHy2.
+  - simpl. constructor. apply IHy.
+Qed.
 
 Theorem _3_21 : forall M M' G, typ_sess M G -> betaP M M' -> exists G', typ_sess M' G' /\ multiC G G'.
 Proof.
@@ -361,12 +524,12 @@ Proof.
         specialize(typable_implies_wfC H5); intros.
         specialize(wfC_recv H26 H23); try easy.
       - apply sc_sub with (s := S); try easy.
-        apply expr_typ_multi with (e := e); try easy.
+        apply expr_typ_step with (e := e); try easy.
         apply sstrans with (s2 := SL'); try easy.
         apply sstrans with (s2 := Sn); try easy. 
         apply sstrans with (s2 := SL); try easy.
       - specialize(guardP_cont_recv_n l xs y q Htt H); intros.
-        specialize(guardP_subst_expr y v 0 0); intros. apply H28; try easy.
+        specialize(guardP_subst_expr y (e_val v) 0 0); intros. apply H28; try easy.
     - constructor.
       specialize(_3_19_1_helper q p l G G' LP LQ SL TL SL' TL'); intros.
       assert(projectionC G' q TL). apply H26; try easy. clear H26.
